New branch, several changes. Baked in the stuff that was in semGen.v

src/Checker.v
@@ -6,8 +6,10 @@ Require Import String.
 Require Import RoseTrees.
 Require Import Show.
 Require Import State.
-Require Import AbstractGen.
+Require Import ModuleGen GenCombinators.
 Require Import Arbitrary.
+
+Import Gen GenComb.
 
 (* Extraction will map this to something that additionally prints stuff *)
 Definition trace (A : Type) (s : string) (a : A) : A := a.
@@ -58,170 +60,163 @@ Record QProp : Type :=
       unProp : Rose Result
     }.
 
-Definition Checker (Gen: Type -> Type) : Type := Gen QProp.
+Definition Checker : Type := G QProp.
 
-Section Checkers.
-  Context {Gen : Type -> Type}
-          {H: GenMonad Gen}.
+Class Checkable (A : Type) : Type :=
+  {
+    checker : A -> Checker
+  }.
 
-  Class Checkable (A : Type) : Type :=
-    {
-      checker : A -> Checker Gen
-    }.
+(* mapping and lifting functions *)
 
-  (* mapping and lifting functions *)
-  
-  Definition liftBool (b : bool) : Result :=
-    if b then succeeded else updReason failed "Falsifiable".
+Definition liftBool (b : bool) : Result :=
+  if b then succeeded else updReason failed "Falsifiable".
 
-  Definition mapProp {P : Type} {_ : Checkable P}
-             (f : QProp -> QProp) (prop : P) : Checker Gen :=
-    fmapGen f (checker prop).
+Definition mapProp {P : Type} {_ : Checkable P}
+           (f : QProp -> QProp) (prop : P) : Checker :=
+  fmap f (checker prop).
 
-  Definition mapRoseResult {P : Type} {_ : Checkable P}
-             (f : Rose Result -> Rose Result) (prop : P) : Checker Gen :=
-    mapProp (fun p => match p with MkProp t => MkProp (f t) end) prop.
+Definition mapRoseResult {P : Type} {_ : Checkable P}
+           (f : Rose Result -> Rose Result) (prop : P) : Checker :=
+  mapProp (fun p => match p with MkProp t => MkProp (f t) end) prop.
 
-  Definition mapTotalResult {prop : Type} {_ : Checkable prop}
-             (f : Result -> Result) : prop -> Checker Gen :=
-    mapRoseResult (fmapRose f).
+Definition mapTotalResult {prop : Type} {_ : Checkable prop}
+           (f : Result -> Result) : prop -> Checker :=
+  mapRoseResult (fmapRose f).
 
-  (* Checkable Instances *)
-  Global Instance testResult : Checkable Result :=
-    {|
-      (* Left a protectResults out! *)
-      checker r := returnGen (MkProp (returnRose r))
-    |}.
-  
+Global Instance testResult : Checkable Result :=
+  {|
+    (* Left a protectResults out! *)
+    checker r := returnGen (MkProp (returnRose r))
+  |}.
 
-  Global Instance testBool : Checkable bool :=
-    {|
-      checker b := checker (liftBool b)
-    |}.
-  
-  (* ZP/CH: what's the relation between unit and discards? *)
-  Global Instance testUnit : Checkable unit :=
-    {|
-      checker := fun _ => checker rejected
-    |}.
 
-  Global Instance testProp : Checkable QProp :=
-    {|
-      checker p := returnGen p
-    |}.
+Global Instance testBool : Checkable bool :=
+  {|
+    checker b := checker (liftBool b)
+  |}.
 
-  Global Instance testGenProp (P : Type) : Checkable P -> Checkable (Gen P) :=
-    {|
-      checker p := bindGen p checker
-    |}.
+(* ZP/CH: what's the relation between unit and discards? *)
+Global Instance testUnit : Checkable unit :=
+  {|
+    checker := fun _ => checker rejected
+  |}.
 
-  
-  (* Checker Combinators *)
-  
-  (* The following function on its own does not have a decreasing argument...
+Global Instance testProp : Checkable QProp :=
+  {|
+    checker p := returnGen p
+  |}.
+
+Global Instance testGenProp (P : Type) : Checkable P -> Checkable (G P) :=
+  {|
+    checker p := bindGen p checker
+  |}.
+
+
+(* Checker Combinators *)
+
+(* The following function on its own does not have a decreasing argument...
 
      Fixpoint props {prop A : Type} {t : Checkable prop}
                     (pf : A -> prop) (shrinker : A -> list A) (x : A) :=
        MkRose (checker (pf x)) (List.map (props pf shrinker) (shrinker x)).
-   *)
-  Fixpoint props' {prop A : Type} {t : Checkable prop} (n : nat)
-           (pf : A -> prop) (shrinker : A -> list A) (x : A) :=
-    match n with
-      | O =>
-        MkRose (checker (pf x)) (lazy nil)
-      | S n' =>
-        MkRose (checker (pf x)) (lazy (List.map (props' n' pf shrinker) (shrinker x)))
-    end.
+ *)
+Fixpoint props' {prop A : Type} {t : Checkable prop} (n : nat)
+         (pf : A -> prop) (shrinker : A -> list A) (x : A) :=
+  match n with
+    | O =>
+      MkRose (checker (pf x)) (lazy nil)
+    | S n' =>
+      MkRose (checker (pf x)) (lazy (List.map (props' n' pf shrinker) (shrinker x)))
+  end.
 
-  (* Arbitrary choice for number of shrinks.. *)
-  Definition props {prop A : Type} `{Checkable prop}
-             (pf : A -> prop) (shrinker : A -> list A) (x : A) : Rose (Checker Gen) :=
-    props' 1000 pf shrinker x.
+(* Arbitrary choice for number of shrinks.. *)
+Definition props {prop A : Type} `{Checkable prop}
+           (pf : A -> prop) (shrinker : A -> list A) (x : A) : Rose Checker :=
+  props' 1000 pf shrinker x.
 
-  Definition shrinking {prop A : Type} `{Checkable prop}
-             (shrinker : A -> list A) (x0 : A) (pf : A -> prop) : Checker Gen :=
-    @fmapGen Gen _ _ _ (fun x => MkProp (joinRose (fmapRose unProp x)))
-             (promote (props pf shrinker x0)).
+Definition shrinking {prop A : Type} `{Checkable prop}
+           (shrinker : A -> list A) (x0 : A) (pf : A -> prop) : Checker :=
+  fmap (fun x => MkProp (joinRose (fmapRose unProp x)))
+       (promote (props pf shrinker x0)).
 
-  Definition callback {prop : Type} `{Checkable prop}
-             (cb : Callback) : prop -> Checker Gen :=
-    mapTotalResult (fun r => addCallback r cb).
+Definition callback {prop : Type} `{Checkable prop}
+           (cb : Callback) : prop -> Checker :=
+  mapTotalResult (fun r => addCallback r cb).
 
-  Definition printTestCase {prop : Type} `{Checkable prop}
-             (s : string) (p : prop) : Checker Gen :=
-    callback (PostFinalFailure Counterexample (fun _st _res => trace s 0)) p.
+Definition printTestCase {prop : Type} `{Checkable prop}
+           (s : string) (p : prop) : Checker :=
+  callback (PostFinalFailure Counterexample (fun _st _res => trace s 0)) p.
 
-  Definition whenFail {prop : Type} `{Checkable prop}
-             (str : string) : prop -> Checker Gen :=
-    callback (PostFinalFailure Counterexample (fun _st _sr => trace str 0)).
+Definition whenFail {prop : Type} `{Checkable prop}
+           (str : string) : prop -> Checker :=
+  callback (PostFinalFailure Counterexample (fun _st _sr => trace str 0)).
 
 
-  Definition expectFailure {prop: Type} `{Checkable prop} (p: prop) := 
-    mapTotalResult (fun res =>
-                      MkResult (ok res) false (reason res) 
+Definition expectFailure {prop: Type} `{Checkable prop} (p: prop) := 
+  mapTotalResult (fun res =>
+                    MkResult (ok res) false (reason res) 
                              (interrupted res) (stamp res) (callbacks res))
-                   p.
+                 p.
 
-  Definition cover {prop : Type} {_ : Checkable prop}
-             (b : bool) (n : nat) (s : string) : prop -> Checker Gen :=
-    if b then
-      mapTotalResult (fun res =>
-                        let '(MkResult o e r i st c) := res in
-                        MkResult o e r i ((s,n)::st) c)
-    else checker.
+Definition cover {prop : Type} {_ : Checkable prop}
+           (b : bool) (n : nat) (s : string) : prop -> Checker :=
+  if b then
+    mapTotalResult (fun res =>
+                      let '(MkResult o e r i st c) := res in
+                      MkResult o e r i ((s,n)::st) c)
+  else checker.
 
-  Definition classify {prop : Type} {_ : Checkable prop}
-             (b : bool) (s : string) : prop -> Checker Gen :=
-    cover b 0 s.
+Definition classify {prop : Type} {_ : Checkable prop}
+           (b : bool) (s : string) : prop -> Checker :=
+  cover b 0 s.
 
-  Definition label {prop : Type} {_ : Checkable prop}
-             (s : string) : prop -> Checker Gen :=
-    classify true s.
+Definition label {prop : Type} {_ : Checkable prop}
+           (s : string) : prop -> Checker :=
+  classify true s.
 
-  Definition collect {A prop : Type} `{_ : Show A} {_ : Checkable prop}
-             (x : A) : prop -> Checker Gen :=
-    label (show x).
-
-
-  Definition implication {prop : Type} `{Checkable prop} (b : bool) (p : prop) :=
-    if b then checker p else checker rejected.
-       
-
-  Definition forAll {A prop : Type} {_ : Checkable prop} `{Show A}
-             (gen : Gen A)  (pf : A -> prop) : Checker Gen :=
-    bindGen gen (fun x =>
-    printTestCase (show x ++ newline) (pf x)).
-
-   Definition forAllShrink {A prop : Type} {_ : Checkable prop} `{Show A}
-              (gen : Gen A) (shrinker : A -> list A) (pf : A -> prop) : Checker Gen :=
-     bindGen gen (fun x =>
-     shrinking shrinker x (fun x' =>
-     printTestCase (show x' ++ newline) (pf x'))).
-
-   Definition forAllShrinkShow {A prop : Type} {_ : Checkable prop}
-              (gen : Gen A) (shrinker : A -> list A) (show' : A -> string) (pf : A -> prop) : Checker Gen :=
-     bindGen gen (fun x =>
-     shrinking shrinker x (fun x' =>
-     printTestCase (show' x' ++ newline) (pf x'))).
-
-  Global Instance testFun {A prop : Type} `{Show A}
-         {_ : Arbitrary A} {_ : Checkable prop} : Checkable (A -> prop) :=
-    {
-      checker f := forAllShrink arbitrary shrink f
-    }.
-
-  Global Instance testPolyFun {prop : Type -> Type} {_ : Checkable (prop nat)} : Checkable (forall T, prop T) :=
-    {
-      checker f := printTestCase "" (f nat)
-    }.
-
-  Global Instance testPolyFunSet {prop : Set -> Type} {_ : Checkable (prop nat)} : Checkable (forall T, prop T) :=
-    {
-      checker f := printTestCase "" (f nat)
-    }.
+Definition collect {A prop : Type} `{_ : Show A} {_ : Checkable prop}
+           (x : A) : prop -> Checker :=
+  label (show x).
 
 
-End Checkers.
+Definition implication {prop : Type} `{Checkable prop} (b : bool) (p : prop) : Checker :=
+  if b then checker p else (returnGen (MkProp (returnRose rejected))).
+
+
+Definition forAll {A prop : Type} {_ : Checkable prop} `{Show A}
+           (gen : G A)  (pf : A -> prop) : Checker :=
+  bindGen gen (fun x =>
+                 printTestCase (show x ++ newline) (pf x)).
+
+Definition forAllShrink {A prop : Type} {_ : Checkable prop} `{Show A}
+           (gen : G A) (shrinker : A -> list A) (pf : A -> prop) : Checker :=
+
+  bindGen gen (fun x : A =>
+                 shrinking shrinker x (fun x' =>
+                                         printTestCase (show x' ++ newline) (pf x'))).
+
+Definition forAllShrinkShow {A prop : Type} {_ : Checkable prop}
+           (gen : G A) (shrinker : A -> list A) (show' : A -> string) (pf : A -> prop) : Checker :=
+  bindGen gen (fun x =>
+                 shrinking shrinker x (fun x' =>
+                                         printTestCase (show' x' ++ newline) (pf x'))).
+
+Global Instance testFun {A prop : Type} `{Show A}
+       {_ : Arbitrary A} {_ : Checkable prop} : Checkable (A -> prop) :=
+  {
+    checker f := forAllShrink arbitrary shrink f
+  }.
+
+Global Instance testPolyFun {prop : Type -> Type} {_ : Checkable (prop nat)} : Checkable (forall T, prop T) :=
+  {
+    checker f := printTestCase "" (f nat)
+  }.
+
+Global Instance testPolyFunSet {prop : Set -> Type} {_ : Checkable (prop nat)} : Checkable (forall T, prop T) :=
+  {
+    checker f := printTestCase "" (f nat)
+  }.
 
 Notation "x ==> y" := (implication x y) (at level 55, right associativity) 
                       : Checker_scope.
