src/SemGen.v
@@ -58,10 +58,8 @@ Infix "--->" := set_incl (at level 70, no associativity) : sem_gen_scope.
 
 Open Scope sem_gen_scope.
 
-Axiom randomSeedInhabitant : RandomGen.
-
 Lemma semReturnSize : forall A (x : A) (size : nat),
-  semSize (returnG x) size <--> eq x.
+  semSize (returnGen x) size <--> eq x.
 Proof.
   move => A x a. rewrite /semSize. split.
   - move => [seed H]. by [].
@@ -70,7 +68,7 @@ Proof.
 Qed.
 
 Lemma semReturn : forall A (x : A),
-  semGen (returnG x) <--> eq x.
+  semGen (returnGen x) <--> eq x.
 Proof. (* this kind of proof should be "trivial by rewriting",
           but this doesn't quite work as easy at it should *)
   move => A x. rewrite /semGen.
@@ -83,17 +81,21 @@ Proof. (* this kind of proof should be "trivial by rewriting",
   - move => H. exists 0. by rewrite G.
 Qed.
 
+
+
+
+
 (* For cardinality reasons this requires RandomGen to be infinite;
    this is just an abstraction of what's happening at the lower levels *)
 Axiom rndSplitAssumption :
   forall s1 s2 : RandomGen, exists s, rndSplit s = (s1,s2).
  
 Lemma semBindSize : forall A B (g : Gen A) (f : A -> Gen B) (size : nat),
-  semSize (bindG g f) size <-->
+  semSize (bindGen g f) size <-->
   fun b => exists a, (semSize g size) a /\
                      (semSize (f a) size) b.
 Proof.
-  move => A B [g] f size b. rewrite /semSize /bindG => /=. split.
+  move => A B [g] f size b. rewrite /semSize /bindGen => /=. split.
   - case => [seed H]. move : H.
     case (rndSplit seed) => [seed1 seed2] H.
     exists (g seed1 size). split; eexists. reflexivity.
@@ -103,11 +105,40 @@ Proof.
     exists seed. rewrite Hseed. rewrite H1. move : H2. by case (f a).
 Qed.
 
+ 
+Lemma semBind : forall A B (g : Gen A) (f : A -> Gen B),
+  semGen (bindGen g f) --->
+  fun b => exists a, (semGen g) a /\
+                     (semGen (f a)) b.
+Proof.
+  move => A B [g] f b [size [seed H]]. rewrite /semSize /bindGen => /=.  
+  simpl in *.
+  destruct (rndSplit seed) as [seed1 seed2]. 
+  subst. exists (g seed1 size).
+  split. by exists size; exists seed1. 
+  exists size. exists seed2. by case: (f (g seed1 size)).
+Qed.
+
+Lemma semBindComb : 
+  forall A B (g : Gen A) (f : A -> Gen B),
+    (fun b => exists a n, (semSize g n) a /\
+                        (semSize (f a) n) b) --->
+  semGen (bindGen g f).
+Proof.
+  move => A B [g] f b [a [n [[seed1 /= H1] [seed2 H2]]]].
+  exists n.
+  case (rndSplitAssumption seed1 seed2) => [seed Hseed].
+  exists seed. simpl. rewrite Hseed. rewrite H1. 
+  by destruct (f a). 
+Qed.
+  
+  
+
 Lemma semFMapSize : forall A B (f : A -> B) (g : Gen A) (size : nat),
-  semSize (fmapG f g) size <-->
+  semSize (fmap f g) size <-->
     (fun b => exists a, (semSize g size) a /\ b = f a).
 Proof.
-  move => A B f [g] size b. rewrite /semSize /fmapG => /=. split.
+  move => A B f [g] size b. rewrite /semSize /fmap => /=. split.
   - move => [seed H]. exists (g seed size). by eauto.
   - move => [a [[seed H1] H2]].
     eexists. rewrite H2. rewrite <- H1. reflexivity.
@@ -115,17 +146,25 @@ Qed.
 
 (* This should just use semFMapSize *)
 Lemma semFMap : forall A B (f : A -> B) (g : Gen A),
-  semGen (fmapG f g) <-->
+  semGen (fmap f g) <-->
     (fun b => exists a, (semGen g) a /\ b = f a).
 Proof.
-  move => A B f [g] b. rewrite /semGen /semSize /fmapG => /=. split.
+  move => A B f [g] b. rewrite /semGen /semSize /fmap => /=. split.
   - move => [size [seed H]]. exists (g seed size). by eauto.
   - move => [a [[size [seed H1]] H2]].
     do 2 eexists. rewrite H2. rewrite <- H1. reflexivity.
 Qed.
 
+Lemma semChooseSize : forall A `{Random A} a1 a2 s,
+  semSize (choose (a1,a2)) s <--> (fun a => Random.leq a1 a /\ Random.leq a a2).
+Proof.
+  move => A R a1 a2 a. rewrite /semGen /semSize. simpl. split.
+  - move => [seed H]. apply randomRCorrect. by exists seed.
+  - by move => /randomRCorrect H.
+Qed.  
+
 Lemma semChoose : forall A `{Random A} a1 a2,
-  semGen (chooseG (a1,a2)) <--> (fun a => Random.leq a1 a /\ Random.leq a a2).
+  semGen (choose (a1,a2)) <--> (fun a => Random.leq a1 a /\ Random.leq a a2).
 Proof.
   move => A R a1 a2 a. rewrite /semGen /semSize. simpl. split.
   - by move => [_ /randomRCorrect H].
@@ -133,14 +172,15 @@ Proof.
 Qed.  
 
 Lemma semSizedSize : forall A (f : nat -> Gen A),
-  semGen (sizedG f) <--> (fun a => exists n, semSize (f n) n a).
+  semGen (sized f) <--> (fun a => exists n, semSize (f n) n a).
 Proof.
-  move => A f a. rewrite /semGen /semSize /sizedG => /=. split.
+  move => A f a. rewrite /semGen /semSize /sized => /=. split.
   - move => [size [seed H]]. exists size. move : H.
     case (f size) => g H. rewrite /semSize. by eauto.
   - move => [size [seed H]]. exists size. exists seed.
     move : H. case (f size) => g H. rewrite /semSize. by eauto.
 Qed.
+
 
 Lemma semResize : forall A (n : nat) (g : Gen A),
   semGen (resize n g) <--> semSize g n .
@@ -156,7 +196,7 @@ Lemma semGenSuchThatMaybeAux_sound:
     (exists size seed, (unGen g) seed size = a) /\ p a.
 Proof. 
   move=> /= A g p k n. elim : n k =>  [//=| n IHn] k a seed size H.
-  simpl in *. unfold unGen, bindG in H.
+  simpl in *. unfold unGen, bindGen in H.
   remember (resize (2 * k + n.+1) g) as g'.
   case: g' H Heqg'=> /= g' H Heqg'.
   case: (rndSplit seed) H Heqg'=> /= r1 r2 H Heqg'. 
@@ -168,19 +208,6 @@ Proof.
   eapply (IHn k.+1 a r2 size). rewrite -H.
   by destruct (suchThatMaybeAux g p k.+1 n).
 Qed.
- 
-(* Lemma semGenSuchThatMaybeAux_complete: *)
-(*   forall {A} g (p : A -> bool) (a : A) seed size, *)
-(*     (unGen g) seed size = a -> p a -> *)
-(*     exists seed size n k,  *)
-(*       unGen (suchThatMaybeAux g p k n) seed size = Some a. *)
-(* Proof.   *)
-(*   move=> A [g] /= p a seed size H pa.  *)
-(*   move/(_ seed seed): rndSplitAssumption => [s Hs]. *)
-(*   exists s. *)
-(*   exists 0. exists (size.+1). exists 0 => //=.  *)
-(*   rewrite Hs /=. by rewrite muln0 add0n H pa. *)
-(* Qed. *)
    
 Lemma semSuchThatMaybe : forall A (g : Gen A) (f : A -> bool),
   semGen (suchThatMaybeG g f) --->
@@ -199,13 +226,10 @@ Proof.
     by destruct (suchThatMaybeAux g f 0 n').
 Qed.
       
-Definition roseRoot {A : Type} (ra : Rose A) : A :=
-  match ra with
-    | MkRose r _ => r
-  end.
 
+(* This is trivial, just the definition *)
 Lemma semPromote : forall A (m : Rose (Gen A)),
-  semGen (promoteG m) <--> 
+  semGen (promote m) <--> 
          fun (t : (Rose A)) => 
            exists seed size, 
               (fmapRose (fun (g : Gen A) => unGen g seed size) m) = t.
@@ -214,6 +238,141 @@ Proof.
   move => [size [seed H]]; exists seed; exists size=> //=. 
 Qed.
 
+(* Semantics for derived generators *)
+
+Lemma semliftGen :
+  forall {A B} (f: A -> B) (g: Gen A),
+    semGen (liftGen f g) <-->
+      fun b =>
+      exists a, semGen g a /\ f a = b.
+Proof. 
+  rewrite /liftGen. move => A B f g b. split.
+  - move => [size /semBindSize [a [H1 H2]]]; subst.
+    exists a. apply semReturnSize in H2. 
+    split => //. by exists size.
+  - move => [a [[size H] Heq]]; subst.
+    exists size. apply semBindSize.
+    exists a. split => //. by apply semReturnSize.
+Qed.
+
+
+Lemma semSize_semGen: 
+  forall {A} (g: Gen A) n, semSize g n ---> semGen g.
+Proof.
+  move => A g n a H. by exists n.
+Qed.
+
+Lemma sequenceGen_equiv :
+  forall {A} (gs : list (Gen A)) n,
+    semSize (sequenceGen gs) n <--> 
+           fun l => length l = length gs /\
+                    forall x, List.In x (combine l gs) -> 
+                              semSize (snd x) n (fst x).
+Proof.
+  move=> A gs n la. rewrite /sequenceGen. split.
+  - elim : gs la => /= [| g gs IHgs] la.
+    + by move/semReturnSize => H; subst. 
+    + move => /semBindSize [a [H1 /semBindSize 
+                                  [la' [H2 /semReturnSize H3]]]]; subst.
+      move: IHgs => /(_ la' H2) [<- HIn].
+      split=> //= x [H | H]; subst => //=. by apply HIn => /=.
+  - elim : gs la => /= [| g gs IHgs].
+    + move => [|a la] [//= Heq H]. 
+      by apply semReturnSize. 
+    + move => [|a la] [//= [Heq] HIn]; subst.
+      apply semBindSize. 
+      exists a. split. 
+      * apply (HIn (a, g)). by left.
+      * apply semBindSize. exists la. 
+        split => //=.
+        apply IHgs. split => // x H. apply HIn; by right.
+        by apply semReturnSize.
+Qed.  
+
+Lemma vectorOf_equiv: 
+  forall {A : Type} (k : nat) (g : Gen A) n,
+    semSize (vectorOf k g) n <--> 
+    fun l => (length l = k /\ forall x, List.In x l -> semSize g n x).
+Proof.
+  move => A k g n la; unfold vectorOf; split.
+  - elim : k la => /= [|k IHk] la.  
+    + move=> /semReturnSize H; subst. by split.
+    + move=> /semBindSize [a [H1 /semBindSize [la' [H2 /semReturnSize H3]]]].
+      subst => /=. 
+      have [<- HIn]: length la' = k /\ (forall x : A, List.In x la' -> semSize g n x)
+        by apply IHk. 
+      split => // x [H | H]; subst => //. 
+      by apply HIn.
+  - elim : k la => /= [|k IHk] la [Heq Hgen]. 
+    + destruct la => //. by apply semReturnSize.
+    + destruct la=> //. simpl in *.
+      move: Heq => [Heq]; subst.
+      apply semBindSize.
+      exists a. split.
+      * apply Hgen => //; by left.
+      * apply semBindSize.
+        exists la =>//. split => //; last by apply semReturnSize.  
+        apply IHk. split => //.
+        move => x HIn. apply Hgen. by right.
+Qed.
+ 
+
+Lemma In_nth_exists:
+  forall {A} (l: list A) x def,
+    List.In x l -> exists n, nth n l def = x /\ (n < length l)%coq_nat.
+Proof.
+   move => A l x def. elim : l => [| a l IHl]  //=. 
+   move => [H | /IHl [n [H1 H2]]]; subst.
+   - exists 0. split => //. omega.
+   - exists n.+1. split => //. omega.
+Qed.
+  
+Lemma oneof_equiv:
+  forall {A} (l : list (Gen A)) (def : Gen A),
+    (semGen (oneof def l)) <-->
+    (fun e => (exists x, List.In x l /\ semGen x e) \/ 
+              (l = nil /\ semGen def e)).
+Proof.
+  move=> A l def a. unfold oneof. split.
+  - move => [s /semBindSize [n [/semChooseSize [Hleq1 Hleq2] Hnth]]]. 
+    case: l Hleq2 Hnth => [| g gs] //= /leP Hleq2 Hnth.
+    + rewrite sub0n in Hleq2. apply le_n_0_eq in Hleq2; subst. 
+      right. split => //. by exists s.
+    + left. rewrite subn1 NPeano.Nat.pred_succ in Hleq2.  
+      case: n Hleq1 Hleq2 Hnth => [_ _ | n Hleq1 Hleq2] Hnth.
+      * exists g. split; auto. by exists s.
+      * exists (nth n gs def). split; last by exists s.
+        right. by apply nth_In.
+  - move => [[g [Hin [s Hsem]]] | [Heq [s Hsem]]]; subst.
+    + exists s. apply semBindSize.  
+      destruct (In_nth_exists _ _ def Hin) as [n [Hnth Hl]]; subst.
+      exists n. split => //. apply semChooseSize. split => //.
+      simpl. apply/leP.
+      rewrite subn1. apply NPeano.Nat.le_succ_le_pred. omega.
+    + exists s. apply semBindSize. exists 0. split => //.
+      apply semChooseSize. split => //.
+Qed.
+
+Lemma elements_equiv :
+  forall {A} (l: list A) (def : A),
+    (semGen (elements def l)) <--> (fun e => List.In e l \/ (l = nil /\ e = def)).
+Proof.
+ unfold elements. move => A l def a. split.
+ - move => [s /semBindSize [n [/semChooseSize [/= Hleq1 Hleq2] 
+                                /semReturnSize H2]]]; subst.
+   case: l Hleq1 Hleq2 => [_ _ | a l /= Hleq1 Hleq2]. 
+   + right. split => //. by case: n.
+   + left. case: n Hleq1 Hleq2 => [|n] _ /leP Hleq2; auto.
+     right. apply nth_In. rewrite subn1 in Hleq2. omega.
+ - move => [H | [H1 H2]]; subst.
+   + exists 0. apply semBindSize. 
+     destruct (In_nth_exists _ _ def H) as [n [Hnth Hlen]]; subst.
+     exists n. split; last by apply semReturnSize.
+     apply semChooseSize. split => //. apply/leP. 
+     unfold lt in *. rewrite subn1. omega.
+   + exists 0. apply semBindSize. exists 0.
+     split; last by apply semReturnSize. apply semChooseSize. split => //. 
+Qed.
 
 (* A proof that shrinking doesn't affect the semantics of testing *)
 (* This should move to the appropriate file, once we propagate the changes *)
@@ -222,8 +381,8 @@ Require Import Checker.
 
 Definition shrinking {prop A : Type} {_: @Checkable Gen.Gen prop}
            (shrinker : A -> list A) (x0 : A) (pf : A -> prop) : Checker Gen :=
-  fmapG (fun x => MkProp (joinRose (fmapRose unProp x)))
-        (promoteG (props pf shrinker x0)).
+  fmap (fun x => MkProp (joinRose (fmapRose unProp x)))
+        (promote (props pf shrinker x0)).
 
 Definition resultSuccessful (r : Result) : bool :=
   match r with
@@ -260,9 +419,9 @@ Proof.
     + suff :
         success
           (unGen
-             (fmapG
+             (fmap
                 (fun x0 => {| unProp := joinRose (fmapRose unProp x0) |})
-                (promoteG (@props' _ _ _ HCheck n.+1 pf sh x))) seed size) = true;
+                (promote (@props' _ _ _ HCheck n.+1 pf sh x))) seed size) = true;
       first by simpl; destruct (unGen (checker (pf x)) seed size) as [[? ?]].
       by apply H; exists size; exists seed.
   - unfold props. generalize 1000.  
