src/GenCombinators.v
@@ -1,0 +1,351 @@
+Require Import ZArith List ssreflect ssrbool ssrnat.
+Require Import Axioms Random ModuleGen.
+Require Import Ensembles.
+
+Import Gen ListNotations.
+
+Module Type GenDerivedInterface.
+  
+  Parameter liftGen : forall {A B : Type}, (A -> B) -> G A -> G B.
+  Parameter liftGen2 : forall {A1 A2 B : Type}, 
+                         (A1 -> A2 -> B) -> G A1 -> G A2 -> G B.
+  Parameter liftGen3 : forall {A1 A2 A3 B : Type}, 
+                         (A1 -> A2 -> A3 -> B) -> G A1 -> G A2 -> G A3 -> G B.
+  Parameter liftGen4 : forall {A1 A2 A3 A4 B : Type}, 
+                         (A1 -> A2 -> A3 -> A4 -> B) -> 
+                         G A1 -> G A2 -> G A3 -> G A4 -> G B.
+  Parameter liftGen5 : forall {A1 A2 A3 A4 A5 B : Type}, 
+                         (A1 -> A2 -> A3 -> A4 -> A5 -> B) -> 
+                         G A1 -> G A2 -> G A3 -> G A4-> G A5 -> G B.
+  Parameter sequenceGen: forall {A : Type}, list (G A) -> G (list A).
+  Parameter foldGen : 
+    forall {A B : Type}, (A -> B -> G A) -> list B -> A -> G A.
+  Parameter oneof : forall {A : Type}, G A -> list (G A) -> G A.
+  Parameter frequency : forall {A : Type}, G A -> list (nat * G A) -> G A.
+  Parameter vectorOf : forall {A : Type}, nat -> G A -> G (list A).
+  Parameter listOf : forall {A : Type}, G A -> G (list A).
+  Parameter elements : forall {A : Type}, A -> list A -> G A.
+
+  (* Correctness for derived generators *)
+  (* We should/(hope to) prove the Axioms in comments - 
+     In some of them we may need semSize instead of semGen *)
+  
+  Axiom semLiftGen :
+    forall {A B} (f: A -> B) (g: G A),
+      semGen (liftGen f g) <-->
+      fun b =>
+        exists a, semGen g a /\ f a = b.
+  
+  (* Axiom semLiftGen2 : *)
+  (*   forall {A1 A2 B} (f: A1 -> A2 -> B) (g1 : G A1) (g2 : G A2), *)
+  (*     semGen (liftGen2 f g1 g2) <--> *)
+  (*     fun b => *)
+  (*       exists a1, *)
+  (*         exists a2, semGen g1 a1 /\ semGen g2 a2 /\ f a1 a2 = b. *)
+
+  (* Axiom semLiftGen3 : *)
+  (* forall {A1 A2 A3 B} (f: A1 -> A2 -> A3 -> B) *)
+  (*        (g1: G A1) (g2: G A2) (g3: G A3), *)
+  (*   semGen (liftGen3 f g1 g2 g3) <--> *)
+  (*   fun b => *)
+  (*     exists a1, semGen g1 a1 /\ *)
+  (*                (exists a2, semGen g2 a2 /\ *)
+  (*                            (exists a3, semGen g3 a3 /\ (f a1 a2 a3) = b)). *)
+
+  (* Axiom liftGen4_def : *)
+  (* forall {A1 A2 A3 A4 B} (f:A1 -> A2 -> A3 -> A4 -> B) *)
+  (*        (g1: G A1) (g2: G A2) (g3: G A3) (g4: G A4), *)
+  (*   semGen (liftGen4 f g1 g2 g3 g4) <--> *)
+  (*   fun b => *)
+  (*     exists a1, semGen g1 a1 /\ *)
+  (*                (exists a2, semGen g2 a2 /\ *)
+  (*                            (exists a3, semGen g3 a3 /\ *)
+  (*                                        (exists a4, semGen g4 a4 /\ *)
+  (*                                                    (f a1 a2 a3 a4) = b))). *)
+
+  (* Axiom liftGen5_def : *)
+  (* forall {A1 A2 A3 A4 A5 B} (f: A1 -> A2 -> A3 -> A4 -> A5 -> B) *)
+  (*        (g1: G A1) (g2: G A2) (g3: G A3) (g4: G A4) (g5: G A5), *)
+  (*   semGen (liftGen5 f g1 g2 g3 g4 g5) = *)
+  (*   fun b => *)
+  (*     exists a1, semGen g1 a1 /\ *)
+  (*                (exists a2, semGen g2 a2 /\ *)
+  (*                            (exists a3, semGen g3 a3 /\ *)
+  (*                                        (exists a4, semGen g4 a4 /\ *)
+  (*                                                    (exists a5, semGen g5 a5 /\ *)
+  (*                                                                (f a1 a2 a3 a4 a5) = b)))). *)
+
+  Axiom semSequenceGenSize:
+    forall {A} (gs : list (G A)) n,
+      semSize (sequenceGen gs) n <--> 
+      fun l => length l = length gs /\
+               forall x, List.In x (combine l gs) -> 
+                         semSize (snd x) n (fst x).
+
+  (* Axiom semFoldGen_left : *)
+  (*   forall {A B : Type} (f : A -> B -> G A) (bs : list B) (a0 : A), *)
+  (*     semGen (foldGen f bs a0) <--> *)
+  (*     fold_left (fun g b => fun x => exists a, g a /\ semGen (f a b) x) bs (eq a0). *)
+  
+  (* Axiom semFoldGen_right : *)
+  (*       forall {A B : Type} (f : A -> B -> G A) (bs : list B) (a0 : A), *)
+  (*         semGen (foldGen f bs a0) <--> *)
+  (*         fun an =>  *)
+  (*           fold_right (fun b p => fun a_prev => exists a, semGen (f a_prev b) a /\ p a)  *)
+  (*                      (eq an) bs a0. *)
+
+  Axiom semOneof:
+    forall {A} (l : list (G A)) (def : G A),
+      (semGen (oneof def l)) <-->
+      (fun e => (exists x, List.In x l /\ semGen x e) \/ 
+                (l = nil /\ semGen def e)).
+
+  (* Axiom frequency_equiv : *)
+  (*   forall {A} (l : list (nat * G A)) (def : G A), *)
+  (*     semGen (frequency def l) <--> *)
+  (*     (fun e => (exists n, exists g, (List.In (n, g) l /\ semGen g e /\ n <> 0)) \/ *)
+  (*               ((l = nil \/ (forall x, List.In x l -> fst x = 0)) /\ semGen def e)). *)
+
+  Axiom semVectorOfSize: 
+    forall {A : Type} (k : nat) (g : G A) n,
+      semSize (vectorOf k g) n <--> 
+      fun l => (length l = k /\ forall x, List.In x l -> semSize g n x).
+  
+  (* Axiom semListOf: *)
+  (*   forall {A : Type} (g : G A), *)
+  (*     semGen (listOf g) <--> fun l => (forall x, List.In x l -> semGen g x). *)
+    
+  Axiom semElements:
+    forall {A} (l: list A) (def : A),
+      (semGen (elements def l)) <--> (fun e => List.In e l \/ (l = nil /\ e = def)).
+  
+  
+End GenDerivedInterface.
+
+Module GenComb : GenDerivedInterface.
+
+
+  Definition liftGen {A B} (f: A -> B) (a : G A)
+  : G B := nosimpl
+               (bindGen a (fun x =>
+                returnGen (f x))).
+
+  Definition liftGen2 {A1 A2 B}
+             (C : A1 -> A2 -> B) (m1 : G A1) (m2  : G A2)
+  : G B:=
+    nosimpl (bindGen m1 (fun x1 => bindGen m2 (fun x2 => returnGen (C x1 x2)))).
+
+  Definition liftGen3 {A1 A2 A3 R} (F : A1 -> A2 -> A3 -> R)
+           (m1 : G A1) (m2 : G A2) (m3 : G A3)
+
+  : G R := nosimpl(
+    bindGen m1 (fun x1 =>
+    bindGen m2 (fun x2 =>
+    bindGen m3 (fun x3 =>
+    returnGen (F x1 x2 x3))))).
+
+  Definition liftGen4 {A1 A2 A3 A4 R}
+             (F : A1 -> A2 -> A3 -> A4 -> R)
+             (m1 : G A1) (m2 : G A2) (m3 : G A3) (m4: G A4)
+  : G R := nosimpl(
+    bindGen m1 (fun x1 =>
+    bindGen m2 (fun x2 =>
+    bindGen m3 (fun x3 =>
+    bindGen m4 (fun x4 =>
+    returnGen (F x1 x2 x3 x4)))))).
+
+  Definition liftGen5 {A1 A2 A3 A4 A5 R}
+             (F : A1 -> A2 -> A3 -> A4 -> A5 -> R)
+             (m1 : G A1) (m2 : G A2) (m3 : G A3) (m4: G A4) (m5 : G A5)
+  : G R := nosimpl(
+    bindGen m1 (fun x1 =>
+    bindGen m2 (fun x2 =>
+    bindGen m3 (fun x3 =>
+    bindGen m4 (fun x4 =>
+    bindGen m5 (fun x5 =>
+    returnGen (F x1 x2 x3 x4 x5))))))).
+
+
+  Definition sequenceGen {A : Type} (ms : list (G A)) : G (list A) :=
+    fold_right (fun m m' => bindGen m  (fun x =>
+                            bindGen m' (fun xs =>
+                            returnGen (x :: xs)))) (returnGen []) ms.
+
+  Fixpoint foldGen {A B : Type} (f : A -> B -> G A) (l : list B) (a : A)
+  : G A := nosimpl(
+    match l with
+      | [] => returnGen a
+      | (x :: xs) => bindGen (f a x) (foldGen f xs)
+    end).
+
+  Definition oneof {A : Type} (def: G A) (gs : list (G A)) : G A :=
+    bindGen (choose (0, length gs - 1))
+            (fun n => nth n gs def).
+
+  Fixpoint replicate {A : Type} (n : nat) (x : A) : list A :=
+    match n with
+      | O    => nil
+      | S n' => cons x (replicate n' x)
+    end.
+
+  Fixpoint pick {A : Type} (def : G A) (n : nat) (xs : list (nat * G A))
+  : nat * G A :=
+    match xs with
+      | nil => (0, def)
+      | (k, x) :: xs =>
+        if (n < k) then (k, x)
+        else pick def (n - k) xs
+    end.
+
+  Definition frequency {A : Type} (def : G A) (gs : list (nat * G A))
+  : G A :=
+    let tot := fold_left (fun t p => t + (fst p)) gs 0 in
+    bindGen (choose (0, tot-1)) (fun n =>
+    @snd _ _ (pick def n gs)).
+
+  Definition vectorOf {A : Type} (k : nat) (g : G A)
+  : G (list A) :=
+    fold_right (fun m m' =>
+                  bindGen m (fun x =>
+                  bindGen m' (fun xs => returnGen (cons x xs)))
+               ) (returnGen nil) (replicate k g).
+
+  Definition listOf {A : Type} (g : G A) : G (list A) := nosimpl
+    (sized (fun n => bindGen (choose (0, n)) (fun k => vectorOf k g))).
+
+  Definition elements {A : Type} (def : A) (l : list A) := nosimpl(
+    let n := length l in
+    bindGen (choose (0, n - 1)) (fun n' =>
+    returnGen (List.nth n' l def))).
+
+  Lemma semLiftGen :
+    forall {A B} (f: A -> B) (g: G A),
+      semGen (liftGen f g) <-->
+      fun b =>
+      exists a, semGen g a /\ f a = b.
+  Proof. 
+    rewrite /liftGen. move => A B f g b. split.
+    - move => [size /semBindSize [a [H1 H2]]]; subst.
+      exists a. apply semReturnSize in H2. 
+      split => //. by exists size.
+   - move => [a [[size H] Heq]]; subst.
+     exists size. apply semBindSize.
+     exists a. split => //. by apply semReturnSize.
+  Qed.
+
+  Lemma semSequenceGenSize :
+    forall {A} (gs : list (G A)) n,
+      semSize (sequenceGen gs) n <--> 
+           fun l => length l = length gs /\
+                    forall x, List.In x (combine l gs) -> 
+                              semSize (snd x) n (fst x).
+  Proof.
+    move=> A gs n la. rewrite /sequenceGen. split.
+    - elim : gs la => /= [| g gs IHgs] la.
+      + by move/semReturnSize => H; subst. 
+      + move => /semBindSize [a [H1 /semBindSize 
+                                  [la' [H2 /semReturnSize H3]]]]; subst.
+        move: IHgs => /(_ la' H2) [<- HIn].
+        split=> //= x [H | H]; subst => //=. by apply HIn => /=.
+    - elim : gs la => /= [| g gs IHgs].
+      + move => [|a la] [//= Heq H]. 
+          by apply semReturnSize. 
+      + move => [|a la] [//= [Heq] HIn]; subst.
+        apply semBindSize. 
+        exists a. split. 
+        * apply (HIn (a, g)). by left.
+        * apply semBindSize. exists la. 
+          split => //=.
+          apply IHgs. split => // x H. apply HIn; by right.
+            by apply semReturnSize.
+  Qed.  
+
+  Lemma semVectorOfSize: 
+    forall {A : Type} (k : nat) (g : G A) n,
+      semSize (vectorOf k g) n <--> 
+              fun l => (length l = k /\ forall x, List.In x l -> semSize g n x).
+  Proof.
+    move => A k g n la; unfold vectorOf; split.
+    - elim : k la => /= [|k IHk] la.  
+      + move=> /semReturnSize H; subst. by split.
+      + move=> /semBindSize [a [H1 /semBindSize [la' [H2 /semReturnSize H3]]]].
+        subst => /=. 
+        have [<- HIn]: length la' = k /\ 
+                       (forall x : A, List.In x la' -> semSize g n x)
+          by apply IHk. 
+      split => // x [H | H]; subst => //. 
+      by apply HIn.
+   - elim : k la => /= [|k IHk] la [Heq Hgen]. 
+     + destruct la => //. by apply semReturnSize.
+     + destruct la=> //. simpl in *.
+       move: Heq => [Heq]; subst.
+       apply semBindSize.
+       exists a. split.
+       * apply Hgen => //; by left.
+       * apply semBindSize.
+         exists la =>//. split => //; last by apply semReturnSize.  
+         apply IHk. split => //.
+         move => x HIn. apply Hgen. by right.
+  Qed.
+ 
+
+  Lemma In_nth_exists:
+    forall {A} (l: list A) x def,
+      List.In x l -> exists n, nth n l def = x /\ (n < length l)%coq_nat.
+  Proof.
+    move => A l x def. elim : l => [| a l IHl] //=. 
+    move => [H | /IHl [n [H1 H2]]]; subst.
+    - exists 0. split => //. omega.
+    - exists n.+1. split => //. omega.
+  Qed.
+  
+  Lemma semOneof:
+    forall {A} (l : list (G A)) (def : G A),
+      (semGen (oneof def l)) <-->
+      (fun e => (exists x, List.In x l /\ semGen x e) \/ 
+                (l = nil /\ semGen def e)).
+  Proof.
+    move=> A l def a. unfold oneof. split.
+    - move => [s /semBindSize [n [/semChooseSize [Hleq1 Hleq2] Hnth]]]. 
+      case: l Hleq2 Hnth => [| g gs] //= /leP Hleq2 Hnth.
+      + rewrite sub0n in Hleq2. apply le_n_0_eq in Hleq2; subst. 
+        right. split => //. by exists s.
+      + left. rewrite subn1 NPeano.Nat.pred_succ in Hleq2.  
+        case: n Hleq1 Hleq2 Hnth => [_ _ | n Hleq1 Hleq2] Hnth.
+        * exists g. split; auto. by exists s.
+        * exists (nth n gs def). split; last by exists s.
+          right. by apply nth_In.
+    - move => [[g [Hin [s Hsem]]] | [Heq [s Hsem]]]; subst.
+      + exists s. apply semBindSize.  
+        destruct (In_nth_exists _ _ def Hin) as [n [Hnth Hl]]; subst.
+        exists n. split => //. apply semChooseSize. split => //.
+        simpl. apply/leP.
+        rewrite subn1. apply NPeano.Nat.le_succ_le_pred. omega.
+      + exists s. apply semBindSize. exists 0. split => //.
+        apply semChooseSize. split => //.
+  Qed.
+
+  Lemma semElements :
+    forall {A} (l: list A) (def : A),
+      (semGen (elements def l)) <--> 
+      (fun e => List.In e l \/ (l = nil /\ e = def)).
+  Proof.
+    unfold elements. move => A l def a. split.
+    - move => [s /semBindSize [n [/semChooseSize [/= Hleq1 Hleq2] 
+                                   /semReturnSize H2]]]; subst.
+      case: l Hleq1 Hleq2 => [_ _ | a l /= Hleq1 Hleq2]. 
+      + right. split => //. by case: n.
+      + left. case: n Hleq1 Hleq2 => [|n] _ /leP Hleq2; auto.
+        right. apply nth_In. rewrite subn1 in Hleq2. omega.
+    - move => [H | [H1 H2]]; subst.
+      + exists 0. apply semBindSize. 
+        destruct (In_nth_exists _ _ def H) as [n [Hnth Hlen]]; subst.
+        exists n. split; last by apply semReturnSize.
+        apply semChooseSize. split => //. apply/leP. 
+        unfold lt in *. rewrite subn1. omega.
+     + exists 0. apply semBindSize. exists 0.
+       split; last by apply semReturnSize. apply semChooseSize. split => //. 
+  Qed.
+
+
+End GenComb.
