src/ModuleGen.v
@@ -1,0 +1,401 @@
+Require Import ZArith List ssreflect ssrbool ssrnat.
+Require Import Axioms RoseTrees Random.
+Require Import Ensembles.
+
+Set Implicit Arguments.
+
+Import ListNotations.
+
+(* Do we want to keep seq_eq, set_incl? There are similar definitions
+      at Ensembles library *)
+Definition set_eq {A} (m1 m2 : Ensemble A) :=
+  forall (a : A), m1 a <-> m2 a.
+
+Infix "<-->" := set_eq (at level 70, no associativity) : sem_gen_scope.
+
+Definition set_incl {A} (m1 m2 : Ensemble A) :=
+  forall (a : A), m1 a -> m2 a.
+
+Infix "--->" := set_incl (at level 70, no associativity) : sem_gen_scope.
+
+Open Scope sem_gen_scope.
+
+Module Type GenPrimitiveInterface.
+   Parameter G : Type -> Type.
+   
+   (* Standard (primitive) generator interface *)
+   Parameter returnGen  : forall {A : Type}, A -> G A. 
+   Parameter bindGen :  forall {A B : Type}, G A -> (A -> G B) -> G B.
+   Parameter run  : forall {A : Type}, G A -> RandomGen -> nat -> A.
+   Parameter fmap : forall {A B : Type}, (A -> B) -> G A -> G B.
+   Parameter sized : forall {A: Type}, (nat -> G A) -> G A.
+   Parameter resize : forall {A: Type}, nat -> G A -> G A.
+   Parameter promote : forall {A : Type}, Rose (G A) -> G (Rose A).  
+   Parameter suchThatMaybe : forall {A : Type}, G A -> (A -> bool) -> 
+                                                G (option A).
+   Parameter choose : forall {A : Type} `{Random A}, (A * A) -> G A. 
+   Parameter sample : forall {A : Type}, G A -> list A.
+   
+
+   (* Set of outcomes definitions *)
+   Parameter semSize : forall {A : Type}, G A -> nat -> Ensemble A.
+
+   Definition semGen {A : Type} (g : G A) : Ensemble A :=
+     fun a => exists size, semSize g size a.
+   
+   Axiom semReturn : 
+     forall A (x : A), semGen (returnGen x) <--> eq x.
+   Axiom semReturnSize : 
+     forall A (x : A) (size : nat), semSize (returnGen x) size <--> eq x.
+
+   Axiom semBindSize : 
+     forall A B (g : G A) (f : A -> G B) (size : nat),
+       semSize (bindGen g f) size <-->
+       fun b => exists a, (semSize g size) a /\
+                          (semSize (f a) size) b.
+
+   Axiom semFmap :
+     forall A B (f : A -> B) (g : G A),
+       semGen (fmap f g) <-->
+       (fun b => exists a, (semGen g) a /\ b = f a).
+   Axiom semFmapSize : 
+     forall A B (f : A -> B) (g : G A) (size : nat),
+       semSize (fmap f g) size <-->
+       (fun b => exists a, (semSize g size) a /\ b = f a).
+
+   Axiom semChoose : 
+     forall A `{Random A} a1 a2,
+       semGen (choose (a1,a2)) <--> 
+       (fun a => Random.leq a1 a /\ Random.leq a a2).
+   Axiom semChooseSize : 
+     forall A `{Random A} a1 a2 (size : nat),
+       semSize (choose (a1,a2)) size <--> 
+       (fun a => Random.leq a1 a /\ Random.leq a a2).
+
+   
+   Axiom semSizedSize : 
+     forall A (f : nat -> G A),
+       semGen (sized f) <--> (fun a => exists n, semSize (f n) n a).
+   
+   Axiom semResize : 
+     forall A (n : nat) (g : G A),
+       semGen (resize n g) <--> semSize g n .
+
+   (* We need an completeness as well - this is not exact *)
+   Axiom semSuchThatMaybe_sound:
+     forall A (g : G A) (f : A -> bool),
+       semGen (suchThatMaybe g f) --->
+       (fun o => o = None \/
+                 (exists y, o = Some y /\ semGen g y /\ f y)).   
+
+   (* This is too concrete, but I need it to prove shrinking. 
+      Does this reveal a weakness in our framework? 
+      Should we try to get rid of this?  *)
+
+   Axiom semPromote : 
+     forall A (m : Rose (G A)),
+       semGen (promote m) <--> 
+       fun (t : (Rose A)) => 
+         exists seed size, 
+          (fmapRose (fun (g : G A) => run g seed size) m) = t.
+   Axiom semPromoteSize : 
+     forall (A : Type) (m : Rose (G A)) n,
+       semSize (promote m) n <-->
+       (fun t : Rose A =>
+          exists (seed : Axioms.RandomGen),
+            fmapRose (fun g : G A => run g seed n) m = t).
+   
+
+   (* These are the two statements we prove about generators *) 
+   Axiom semGenCorrect :
+     forall A (g : G A) (x : A),
+         semGen g x <-> exists size seed, run g seed size = x.
+
+
+   (* Those are too concrete, but I need them to prove shrinking. 
+      Does this reveal a weakness in our framework? 
+      Should we try to get rid of this?  
+      This is expected since the spec of promote is too concrete. *)
+
+   Axiom runFmap :
+     forall (A B : Type) (f : A -> B) (g : G A) seed size b,
+       run (fmap f g) seed size = b  <->
+       (exists a : A, run g seed size = a /\ b = f a).
+   Axiom runPromote : 
+     forall A (m : Rose (G A)) seed size o,
+       run (promote m) seed size = o <->   
+       (fmapRose (fun (g : G A) => run g seed size) m) = o.
+
+End GenPrimitiveInterface.
+
+Module Gen : GenPrimitiveInterface.
+  
+   Inductive GenType (A : Type) : Type :=
+   | MkGen : (RandomGen -> nat -> A (** RandomGen*)) -> GenType A.
+
+   Definition G := GenType.
+
+   Definition run {A : Type} (g : G A) : RandomGen -> nat -> A :=
+     match g with MkGen f => f end.
+
+   Definition returnGen {A : Type} (x : A) : G A :=
+     MkGen (fun _ _ => x).
+   
+   Definition bindGen {A B : Type} (g : G A) (k : A -> G B) : G B :=
+     MkGen (fun r n =>
+              let (r1,r2) := rndSplit r in
+               run (k (run g r1 n)) r2 n).
+
+   Definition fmap {A B : Type} (f : A -> B) (g : G A) : G B :=
+     MkGen (fun r n => f ((run g) r n)).
+
+   Definition sized {A : Type} (f : nat -> G A) : G A :=
+     MkGen (fun r n => match f n with MkGen m => m r n end).
+
+   Definition resize {A : Type} (n : nat) (g : G A) : G A :=
+     match g with
+       | MkGen m => MkGen (fun r _ => m r n)
+     end.
+   
+   Definition promote {A : Type} (m : Rose (G A)) : G (Rose A) :=
+     MkGen (fun r n => fmapRose (fun g => run g r n) m).
+   
+   (* ZP: Split suchThatMaybe into two different functions 
+        to make a proof easier *) 
+   Definition suchThatMaybeAux {A : Type} (g : G A) (p : A -> bool) :=
+     fix aux (k : nat) (n : nat) : G (option A) :=
+     match n with
+       | O => returnGen None
+       | S n' =>
+         bindGen (resize (2 * k + n) g) (fun x =>
+                                           if p x then returnGen (Some x)
+                                           else aux (S k) n')
+     end.
+
+   Definition suchThatMaybe {A : Type} (g : G A) (p : A -> bool)
+   : G (option A) :=
+     sized (fun x => suchThatMaybeAux g p 0 (max 1 x)).
+
+   Fixpoint rnds (rnd : RandomGen) (n' : nat) : list RandomGen :=
+     match n' with
+       | O => nil
+       | S n'' =>
+         let (rnd1, rnd2) := rndSplit rnd in
+         cons rnd1 (rnds rnd2 n'')
+     end.
+   
+   Fixpoint createRange (n : nat) (acc : list nat) : list nat :=
+     match n with
+       | O => List.rev (cons O acc)
+       | S n' => createRange n' (cons n acc)
+     end.
+
+   Definition choose {A : Type} `{Random A} (range : A * A) : G A := 
+     MkGen (fun r _ => fst (randomR range r)).
+
+   Definition sample (A : Type) (g : G A) : list A :=
+     match g with
+       | MkGen m =>
+         let rnd := mkRandomGen 0 in
+         let l := List.combine (rnds rnd 20) (createRange 20 nil) in
+         List.map (fun (p : RandomGen * nat) => let (r,n) := p in m r n) l
+     end.
+
+   Definition semSize {A : Type} (g : G A) (size : nat) : Ensemble A :=
+     fun a => exists seed, run g seed size = a.
+
+   Definition semGen {A : Type} (g : G A) : Ensemble A :=
+     fun a => exists size, semSize g size a.
+   
+   Lemma semReturnSize : 
+     forall A (x : A) (size : nat),
+       semSize (returnGen x) size <--> eq x.
+   Proof.
+     move => A x a. rewrite /semSize. split.
+     - move => [seed H]. by [].
+     - move => H /=. rewrite H.
+       exists randomSeedInhabitant. reflexivity.
+   Qed.
+
+   Lemma semReturn : forall A (x : A),
+                       semGen (returnGen x) <--> eq x.
+   Proof. (* this kind of proof should be "trivial by rewriting",
+          but this doesn't quite work as easy at it should *)
+     move => A x. rewrite /semGen.
+     (* was hoping to do the rest by rewriting: setoid_rewrite semReturnSize. *)
+     pose proof (semReturnSize x) as G. unfold set_eq in G.
+     (* setoid_rewrite G. -- failed constraints *)
+     move => a /=. split.
+     - move => [size H]. (* or rewrite -> G in H. exact H. *)
+       rewrite <- G. exact H.
+     - move => H. exists 0. by rewrite G.
+   Qed.
+
+   Lemma semBindSize : forall A B (g : G A) (f : A -> G B) (size : nat),
+                         semSize (bindGen g f) size <-->
+                                 fun b => exists a, (semSize g size) a /\
+                                                    (semSize (f a) size) b.
+   Proof.
+     move => A B [g] f size b. rewrite /semSize /bindGen => /=. split.
+     - case => [seed H]. move : H.
+       case (rndSplit seed) => [seed1 seed2] H.
+       exists (g seed1 size). split; eexists. reflexivity.
+       rewrite <- H. case (f (g seed1 size)). reflexivity.
+     - move => [a [[seed1 H1] [seed2 H2]]].
+       case (rndSplitAssumption seed1 seed2) => [seed Hseed].
+       exists seed. rewrite Hseed. rewrite H1. move : H2. by case (f a).
+   Qed.
+
+   Lemma semFmapSize : forall A B (f : A -> B) (g : G A) (size : nat),
+                         semSize (fmap f g) size <-->
+                                 (fun b => exists a, (semSize g size) a /\ b = f a).
+   Proof.
+     move => A B f [g] size b. rewrite /semSize /fmap => /=. split.
+     - move => [seed H]. exists (g seed size). by eauto.
+     - move => [a [[seed H1] H2]].
+       eexists. rewrite H2. rewrite <- H1. reflexivity.
+   Qed.
+
+   (* This should just use semFMapSize *)
+   Lemma semFmap : forall A B (f : A -> B) (g : G A),
+                     semGen (fmap f g) <-->
+                            (fun b => exists a, (semGen g) a /\ b = f a).
+   Proof.
+     move => A B f [g] b. rewrite /semGen /semSize /fmap => /=. split.
+     - move => [size [seed H]]. exists (g seed size). by eauto.
+     - move => [a [[size [seed H1]] H2]].
+       do 2 eexists. rewrite H2. rewrite <- H1. reflexivity.
+   Qed.
+
+   Lemma semChooseSize : 
+     forall A `{Random A} a1 a2 s,
+       semSize (choose (a1,a2)) s <--> 
+       (fun a => Random.leq a1 a /\ Random.leq a a2).
+   Proof.
+     move => A R a1 a2 a. rewrite /semGen /semSize. simpl. split.
+     - move => [seed H]. apply randomRCorrect. by exists seed.
+     - by move => /randomRCorrect H.
+   Qed.  
+
+   Lemma semChoose : 
+     forall A `{Random A} a1 a2,
+       semGen (choose (a1,a2)) <--> 
+       (fun a => Random.leq a1 a /\ Random.leq a a2).
+   Proof.
+     move => A R a1 a2 a. rewrite /semGen /semSize. simpl. split.
+     - by move => [_ /randomRCorrect H].
+     - move => /randomRCorrect H. by exists 0.
+   Qed.  
+
+   
+   Lemma semSizedSize : 
+     forall A (f : nat -> G A),
+       semGen (sized f) <--> (fun a => exists n, semSize (f n) n a).
+   Proof.
+     move => A f a. rewrite /semGen /semSize /sized => /=. split.
+     - move => [size [seed H]]. exists size. move : H.
+       case (f size) => g H. rewrite /semSize. by eauto.
+     - move => [size [seed H]]. exists size. exists seed.
+       move : H. case (f size) => g H. rewrite /semSize. by eauto.
+   Qed.
+
+
+   Lemma semResize : 
+     forall A (n : nat) (g : G A), semGen (resize n g) <--> semSize g n .
+   Proof.
+     move => A n [g] a. rewrite /semGen /semSize /resize => /=. split.
+     - move => [_ [seed H]]. by eauto.
+     - move => [seed H]. exists 0. by eauto.
+   Qed.
+   
+   Lemma semGenSuchThatMaybeAux_sound:
+     forall {A} g p k n (a : A) seed size,
+       run (suchThatMaybeAux g p k n) seed size = Some a ->
+       (exists size seed, run g seed size = a) /\ p a.
+   Proof. 
+     move=> /= A g p k n. elim : n k =>  [//=| n IHn] k a seed size H.
+     simpl in *. unfold run, bindGen in H.
+     remember (resize (2 * k + n.+1) g) as g'.
+     case: g' H Heqg'=> /= g' H Heqg'.
+     case: (rndSplit seed) H Heqg'=> /= r1 r2 H Heqg'. 
+     remember (p (g' r1 size)) as b.
+     case: b H Heqb => /= H Heqb. inversion H; subst.
+     rewrite /resize in Heqg'.
+     destruct g as [g]. inversion Heqg'; subst.
+     split =>  //=. by eexists; eexists.
+     eapply (IHn k.+1 a r2 size). rewrite -H.
+       by destruct (suchThatMaybeAux g p k.+1 n).
+   Qed.
+
+
+   Lemma semSuchThatMaybe_sound : 
+     forall A (g : G A) (f : A -> bool),
+       semGen (suchThatMaybe g f) --->
+       (fun o => o = None \/
+                 (exists y, o = Some y /\ semGen g y /\ f y)).
+   (* Not an exact spec !!! *)
+   Proof.  
+     move => A g f a. rewrite /semGen /semSize. 
+     - case : a => [a|] [n [s H]]; last by left. right.
+       eexists; split=> //=.
+                          remember (match n with
+                                      | 0 => 1
+                                      | m'.+1 => m'.+1
+                                    end) as n'.  
+       apply (semGenSuchThatMaybeAux_sound g f 0 n' s n). rewrite -H /= -Heqn'.
+         by destruct (suchThatMaybeAux g f 0 n').
+   Qed.
+
+   Lemma semPromote : 
+     forall A (m : Rose (G A)),
+       semGen (promote m) <--> 
+       fun (t : (Rose A)) => 
+         exists seed size, 
+           (fmapRose (fun (g : G A) => run g seed size) m) = t.
+   Proof.  
+     move => A rg r. split; 
+     move => [size [seed H]]; exists seed; exists size=> //=. 
+   Qed.
+
+   Lemma semPromoteSize
+   : forall (A : Type) (m : Rose (G A)) n,
+       semSize (promote m) n <-->
+               (fun t : Rose A =>
+                  exists (seed : Axioms.RandomGen),
+                    fmapRose (fun g : G A => run g seed n) m = t).
+   Proof. 
+     move => A rg r. split; 
+     move => [seed H]; exists seed=> //=. 
+   Qed.
+   
+   (* Those are too concrete, but I need them to prove shrinking. 
+      Does this reveal a weakness in our framework? 
+      Should we try to get rid of this?  
+      This is expected since the spec of promote is too concrete.
+    *)
+   Lemma runFmap :
+     forall (A B : Type) (f : A -> B) (g : G A) seed size b,
+       run (fmap f g) seed size = b  <->
+       (exists a : A, run g seed size = a /\ b = f a).
+   Proof.
+     move => A B f g seed size b'. split => /=.
+     - move => <-. eexists; split => //.
+     - by move => [a [Heq1 Heq2]]; subst.
+   Qed.
+    
+   Lemma runPromote : 
+     forall A (m : Rose (G A)) seed size o,
+       run (promote m) seed size = o <->   
+       (fmapRose (fun (g : G A) => run g seed size) m) = o.
+   Proof.
+     move => A g x. split => //=.
+   Qed.
+
+   Lemma semGenCorrect :
+     forall A (g : G A) (x : A),
+       semGen g x <-> exists size seed, run g seed size = x.
+   Proof.
+     move => A g x. split => //=.
+   Qed.
+
+End Gen.
